prove direct return arg runtime behavior

lowering/defs/evalCompilerRuntimeScript.sml
@@ -1,13 +1,16 @@
 Theory evalCompilerRuntime
 Ancestors
   byte finite_map finite_set list option pair words
-  vfmContext vfmExecution vfmState vfmTransaction vfmCompute[ignore_grammar]
+  vfmConstants vfmContext vfmExecution vfmOperation vfmState vfmTransaction
+  vfmTypes vfmCompute[ignore_grammar]
 Libs
   cv_transLib evalCompilerBytecodeLib finite_mapLib wordsLib
 
 (* TOP-LEVEL:
  *   run_runtime_steps       -- execute bytecode in a minimal single-frame state
  *   run_runtime_steps_from  -- same, with an explicit initial program counter
+ *   direct_return_arg_runtime_call
+ *                           -- parametric calldata-to-return runtime check
  *)
 
 Definition runtime_caller_def:
@@ -117,6 +120,32 @@ End
 
 val () = cv_auto_trans runtime_state_def;
 
+Definition runtime_context_with_def:
+  runtime_context_with pc stack memory returnData gasUsed code calldata =
+    (runtime_context_at pc code calldata) with
+      <| stack := stack; memory := memory;
+         returnData := returnData; gasUsed := gasUsed |>
+End
+
+Definition runtime_state_with_def:
+  runtime_state_with pc stack memory returnData gasUsed code calldata =
+    <| contexts :=
+         [(runtime_context_with pc stack memory returnData gasUsed code calldata,
+           runtime_rollback)];
+       txParams := runtime_tx_params;
+       rollback := runtime_rollback;
+       msdomain := Collect empty_domain
+    |>
+End
+
+Theorem runtime_state_at_0:
+  runtime_state_at 0 code calldata =
+    runtime_state_with 0 [] [] [] 0 code calldata
+Proof
+  simp[runtime_state_at_def, runtime_state_with_def, runtime_context_with_def,
+       runtime_context_at_def, runtime_context_def]
+QED
+
 Definition run_steps_def:
   run_steps 0 s = NONE ∧
   run_steps (SUC fuel) s =
@@ -126,6 +155,8 @@ Definition run_steps_def:
 End
 
 val () = cv_auto_trans run_steps_def;
+
+val run_steps_compute_thm = DB.fetch "-" "run_steps_compute";
 
 Definition run_runtime_steps_from_def:
   run_runtime_steps_from fuel pc code calldata =
@@ -157,4 +188,185 @@ Theorem direct_return_uint_runtime_call:
     SOME (NONE, word_to_bytes_be (1w : bytes32))
 Proof
   CONV_TAC cv_eval
+QED
+
+Definition direct_return_arg_runtime_code_def:
+  direct_return_arg_runtime_code =
+    SND ^(evalCompilerBytecodeLib.read_hex_bytes "direct_return_arg.hex")
+End
+
+val () = cv_trans_deep_embedding EVAL direct_return_arg_runtime_code_def;
+
+Theorem direct_return_arg_runtime_code_bytes:
+  direct_return_arg_runtime_code =
+    [0x5Fw; 0x35w; 0x5Fw; 0x52w; 0x36w; 0x5Fw; 0xF3w]
+Proof
+  CONV_TAC cv_eval
+QED
+
+Theorem direct_return_arg_runtime_parsed:
+  parse_code 0 FEMPTY direct_return_arg_runtime_code =
+    FEMPTY |+ (0, Push 0 []) |+ (1, CallDataLoad) |+
+      (2, Push 0 []) |+ (3, MStore) |+ (4, CallDataSize) |+
+      (5, Push 0 []) |+ (6, Return)
+Proof
+  CONV_TAC cv_eval
+QED
+
+Theorem word_of_bytes_be_word_to_bytes_be_256:
+  word_of_bytes_be (word_to_bytes_be (w : bytes32)) = w
+Proof
+  simp[word_to_bytes_be_def, word_of_bytes_be_def,
+       word_of_bytes_word_to_bytes]
+QED
+
+Theorem LENGTH_word_to_bytes_be_256:
+  LENGTH (word_to_bytes_be (w : bytes32)) = 32
+Proof
+  simp[word_to_bytes_be_def, LENGTH_word_to_bytes]
+QED
+
+Theorem word_to_bytes_be_reverse_le:
+  ∀v:'a word. word_to_bytes v T = REVERSE (word_to_bytes v F)
+Proof
+  simp[GSYM word_to_bytes_be_def, GSYM word_to_bytes_le_def,
+       cv_stdTheory.word_to_bytes_be_eq_bytes_of_num,
+       cv_stdTheory.word_to_bytes_le_eq_bytes_of_num]
+QED
+
+Theorem call_data_load_word_to_bytes_be:
+  word_of_bytes F 0w
+    (REVERSE (take_pad_0 32 (word_to_bytes_be (w : bytes32)))) = w
+Proof
+  `LENGTH (REVERSE (word_to_bytes (w : bytes32) F)) = 32` by
+    simp[LENGTH_word_to_bytes] >>
+  simp[take_pad_0_def, word_to_bytes_be_def, LENGTH_word_to_bytes,
+       word_to_bytes_be_reverse_le, TAKE_LENGTH_TOO_LONG, PAD_RIGHT,
+       word_of_bytes_word_to_bytes]
+QED
+
+Theorem mstore_word_to_bytes_be:
+  REVERSE (word_to_bytes (w : bytes32) F) = word_to_bytes_be w
+Proof
+  simp[word_to_bytes_be_def, word_to_bytes_be_reverse_le]
+QED
+
+val direct_return_arg_step_defs = [
+  step_def, handle_def, bind_def, return_def, fail_def, assert_def,
+  get_current_context_def, set_current_context_def, get_call_data_def,
+  runtime_state_with_def, runtime_context_with_def, runtime_context_at_def,
+  runtime_context_def, runtime_msg_params_def, direct_return_arg_runtime_parsed,
+  direct_return_arg_runtime_code_bytes, empty_return_destination_def,
+  FLOOKUP_UPDATE, step_inst_def,
+  step_push_def, step_call_data_load_def, step_mstore_def, step_msgParams_def,
+  step_context_def, step_return_def, consume_gas_def, push_stack_def,
+  pop_stack_def, memory_expansion_info_def, memory_expansion_cost_def,
+  memory_cost_def, memory_cost_per_word_def, word_size_def, expand_memory_def,
+  write_memory_def, read_memory_def, set_return_data_def, finish_def, handle_step_def,
+  handle_create_def, handle_exception_def, get_return_data_def,
+  get_output_to_def, get_num_contexts_def, reraise_def, vfm_abort_def,
+  inc_pc_or_jump_def,
+  ignore_bind_def, is_call_def, LET_THM, opcode_def, word_of_bytes_def,
+  mstore_word_to_bytes_be, call_data_load_word_to_bytes_be,
+  LENGTH_word_to_bytes_be_256, LENGTH_word_to_bytes, TAKE_LENGTH_TOO_LONG
+];
+
+Theorem direct_return_arg_step_push0_offset:
+  step (runtime_state_with 0 [] [] [] 0 direct_return_arg_runtime_code
+          (word_to_bytes_be (w : bytes32))) =
+    (INL (),
+     runtime_state_with 1 [0w] [] [] 2 direct_return_arg_runtime_code
+       (word_to_bytes_be w))
+Proof
+  simp direct_return_arg_step_defs
+QED
+
+Theorem direct_return_arg_step_calldataload:
+  step (runtime_state_with 1 [0w] [] [] 2 direct_return_arg_runtime_code
+          (word_to_bytes_be (w : bytes32))) =
+    (INL (),
+     runtime_state_with 2 [w] [] [] 5 direct_return_arg_runtime_code
+       (word_to_bytes_be w))
+Proof
+  simp direct_return_arg_step_defs
+QED
+
+Theorem direct_return_arg_step_push0_mstore_offset:
+  step (runtime_state_with 2 [w] [] [] 5 direct_return_arg_runtime_code
+          (word_to_bytes_be (w : bytes32))) =
+    (INL (),
+     runtime_state_with 3 [0w; w] [] [] 7 direct_return_arg_runtime_code
+       (word_to_bytes_be w))
+Proof
+  simp direct_return_arg_step_defs
+QED
+
+Theorem direct_return_arg_step_mstore:
+  step (runtime_state_with 3 [0w; w] [] [] 7 direct_return_arg_runtime_code
+          (word_to_bytes_be (w : bytes32))) =
+    (INL (),
+     runtime_state_with 4 [] (word_to_bytes_be w) [] 13
+       direct_return_arg_runtime_code (word_to_bytes_be w))
+Proof
+  simp direct_return_arg_step_defs
+QED
+
+Theorem direct_return_arg_step_calldatasize:
+  step (runtime_state_with 4 [] (word_to_bytes_be w) [] 13
+          direct_return_arg_runtime_code (word_to_bytes_be (w : bytes32))) =
+    (INL (),
+     runtime_state_with 5 [32w] (word_to_bytes_be w) [] 15
+       direct_return_arg_runtime_code (word_to_bytes_be w))
+Proof
+  simp direct_return_arg_step_defs
+QED
+
+Theorem direct_return_arg_step_push0_return_offset:
+  step (runtime_state_with 5 [32w] (word_to_bytes_be w) [] 15
+          direct_return_arg_runtime_code (word_to_bytes_be (w : bytes32))) =
+    (INL (),
+     runtime_state_with 6 [0w; 32w] (word_to_bytes_be w) [] 17
+       direct_return_arg_runtime_code (word_to_bytes_be w))
+Proof
+  simp direct_return_arg_step_defs
+QED
+
+Theorem direct_return_arg_step_return:
+  step (runtime_state_with 6 [0w; 32w] (word_to_bytes_be w) [] 17
+          direct_return_arg_runtime_code (word_to_bytes_be (w : bytes32))) =
+    (INR NONE,
+     runtime_state_with 6 [] (word_to_bytes_be w) (word_to_bytes_be w) 17
+       direct_return_arg_runtime_code (word_to_bytes_be w))
+Proof
+  simp direct_return_arg_step_defs
+QED
+
+Theorem direct_return_arg_run_steps:
+  run_steps 16
+    (runtime_state_with 0 [] [] [] 0 direct_return_arg_runtime_code
+       (word_to_bytes_be (w : bytes32))) =
+    SOME (NONE,
+      runtime_state_with 6 [] (word_to_bytes_be w) (word_to_bytes_be w) 17
+        direct_return_arg_runtime_code (word_to_bytes_be w))
+Proof
+  simp[run_steps_compute_thm,
+       direct_return_arg_step_push0_offset,
+       direct_return_arg_step_calldataload,
+       direct_return_arg_step_push0_mstore_offset,
+       direct_return_arg_step_mstore,
+       direct_return_arg_step_calldatasize,
+       direct_return_arg_step_push0_return_offset,
+       direct_return_arg_step_return]
+QED
+
+Theorem direct_return_arg_runtime_call:
+  ∀w.
+    run_runtime_steps 16 direct_return_arg_runtime_code
+      (word_to_bytes_be (w : bytes32)) =
+      SOME (NONE, word_to_bytes_be w)
+Proof
+  simp[run_runtime_steps_def, run_runtime_steps_from_def,
+       runtime_state_at_0] >>
+  simp[direct_return_arg_run_steps] >>
+  simp[runtime_state_with_def, runtime_context_with_def]
 QED
